src/spec/properties/TLS13.Wire.Spec.Reveal.Alert.fsti
@@ -1,28 +1,18 @@
 module TLS13.Wire.Spec.Reveal.Alert
 
 module B = TLS13.Bytes
+module GA = TLS13.Wire.Generated.Alert
+module LP = LowParse.Spec
 module M = TLS13.Messages
-module Seq = FStar.Seq
 module T = TLS13.Types
-module U8 = FStar.UInt8
 module WS = TLS13.Wire.Spec
 
 val lemma_ptm_alert:
   fragment:B.bytes ->
-  Lemma (ensures (
-    if B.length fragment == 2
-    then
-      WS.parse_tls_message T.Alert fragment ==
-        (match U8.v (Seq.index fragment 1) with
-         | 0   -> Some (M.TlsAlert T.Close_notify)
-         | 10  -> Some (M.TlsAlert T.Unexpected_message)
-         | 20  -> Some (M.TlsAlert T.Bad_record_mac)
-         | 40  -> Some (M.TlsAlert T.Handshake_failure)
-         | 46  -> Some (M.TlsAlert T.Certificate_unknown)
-         | 47  -> Some (M.TlsAlert T.Illegal_parameter)
-         | 50  -> Some (M.TlsAlert T.Decode_error)
-         | 51  -> Some (M.TlsAlert T.Decrypt_error)
-         | 70  -> Some (M.TlsAlert T.Protocol_version)
-         | 110 -> Some (M.TlsAlert T.Unsupported_extension)
-         | _   -> None)
-    else WS.parse_tls_message T.Alert fragment == None))
+  Lemma (ensures WS.parse_tls_message T.Alert fragment ==
+    (match LP.parse GA.alert_parser fragment with
+     | Some (alert, consumed) ->
+       if consumed == B.length fragment
+       then Some (M.TlsAlert alert.GA.description)
+       else None
+     | None -> None))
